src/SepAuto.v
@@ -891,6 +891,7 @@ Ltac cancel_with t :=
       | [ |- _ =p=> _ ] => cancel'
       end;
   intuition;
+  try eauto;
   try ( pred_apply; cancel_with t );
   try congruence;
   try t;
